theories/Semantics/IMP/Algebraic.v
@@ -1,0 +1,414 @@
+From stdpp Require Import prelude.
+From sets Require Import Ensemble.
+From Semantics Require Import Syntax State Denotational.
+
+Record signature : Type := {
+sort : Type;
+symbols : Type;
+result_sort : symbols -> sort;
+arity : symbols -> { n : nat & fin n -> sort};
+}.
+
+Arguments result_sort {s} _: assert.
+Arguments arity {s} _: assert.
+
+Definition support_star_helper `(support : sort Sigma -> Type)
+    `(ar : fin n -> sort Sigma) : Type :=
+    forall (i : fin n), support (ar i).
+
+Record algebra (Sigma : signature) : Type := {
+support : sort Sigma -> Type;
+support_star `(ar : fin n -> sort Sigma) : Type :=
+    support_star_helper support ar;
+op_interp :
+    forall (sigma : symbols Sigma)
+        (tuple : support_star (projT2 (arity sigma))),
+        support (result_sort sigma);
+}.
+
+Arguments support {Sigma} a _ : assert.
+Arguments support_star {Sigma} a {n}%nat_scope ar%function_scope : assert.
+Arguments op_interp {Sigma} a sigma tuple : assert.
+
+Section sec_sigma_algebra.
+
+Context
+  {Sigma : signature}.
+
+Definition algebra_fn (A B : algebra Sigma): Type :=
+    forall (s : sort Sigma), support A s -> support B s.
+
+Definition algebra_fn_id (A : algebra Sigma): algebra_fn A A :=
+    fun (s : sort Sigma) => id.
+
+Definition algebra_fn_compose {A B C : algebra Sigma}
+    (g : algebra_fn B C) (f : algebra_fn A B) : algebra_fn A C :=
+    fun (s : sort Sigma) => g s ∘ f s.
+
+Lemma algebra_fn_compose_id_left:
+    forall (A B : algebra Sigma) (f : algebra_fn A B),
+    algebra_fn_compose (algebra_fn_id B) f = f.
+Proof. done. Qed.
+
+Lemma algebra_fn_compose_id_right:
+    forall (A B : algebra Sigma) (f : algebra_fn A B),
+    algebra_fn_compose f (algebra_fn_id A) = f.
+Proof. done. Qed.
+
+Lemma algebra_fn_compose_assoc: forall (A B C D : algebra Sigma)
+    (f : algebra_fn A B) (g : algebra_fn B C) (h : algebra_fn C D),
+    algebra_fn_compose h (algebra_fn_compose g f)
+      =
+    algebra_fn_compose (algebra_fn_compose h g) f.
+Proof. done. Qed.
+
+Definition algebra_fn_star `(f : algebra_fn A B) `{ar : fin n -> sort Sigma}
+  (a_star : support_star A ar): support_star B ar :=
+  fun i => (f (ar i) (a_star i)).
+
+Class AlgebraMorphism `(f : algebra_fn A B): Prop :=
+  algebra_morphism : forall (sigma : symbols Sigma) (a_star : support_star A (projT2 (arity sigma))),
+    f (result_sort sigma) (op_interp A sigma a_star)
+      =
+    op_interp B sigma (algebra_fn_star f a_star).
+
+#[export] Instance algebra_fn_id_morphism:
+    forall (A : algebra Sigma), AlgebraMorphism (algebra_fn_id A).
+Proof. done. Qed.
+
+#[export] Instance algebra_fn_compose_morphism:
+    forall (A B C : algebra Sigma) (g : algebra_fn B C) (f : algebra_fn A B),
+    AlgebraMorphism f -> AlgebraMorphism g ->
+    AlgebraMorphism (algebra_fn_compose g f).
+Proof.
+    intros * Hf Hg ? ?; unfold algebra_fn_compose at 1; cbn.
+    by rewrite Hf, Hg.
+Qed.
+
+Class AlgebraIso `(f : algebra_fn A B) (g : algebra_fn B A) : Prop :=
+{
+    f_morphism :> AlgebraMorphism f;
+    g_morphism :> AlgebraMorphism g;
+    algebra_iso_A : algebra_fn_compose g f = algebra_fn_id A;
+    algebra_iso_B : algebra_fn_compose f g = algebra_fn_id B;
+}.
+
+Class Initial (A : algebra Sigma) : Prop :=
+    initiality :
+      forall (B : algebra Sigma), exists! (f : algebra_fn A B), AlgebraMorphism f.
+
+#[export] Instance equiv_algebra : Equiv (algebra Sigma) :=
+    fun A B => exists (f : algebra_fn A B) (g : algebra_fn B A), AlgebraIso f g.
+
+Lemma initial_algebras_iso:
+    forall (A B : algebra Sigma), Initial A -> Initial B -> A ≡ B.
+Proof.
+    intros A B HA HB.
+    destruct (HA B) as (f & Hf & _).
+    destruct (HB A) as (g & Hg & _).
+    exists f, g; split; [done | done |..].
+    - destruct (HA A) as (ida & Hida & Hunida).
+      rewrite <- (Hunida (algebra_fn_id A)) by typeclasses eauto.
+      by symmetry; apply Hunida; typeclasses eauto.
+    - destruct (HB B) as (idb & Hidb & Hunidb).
+      rewrite <- (Hunidb (algebra_fn_id B)) by typeclasses eauto.
+      by symmetry; apply Hunidb; typeclasses eauto.
+Qed.
+
+Lemma Initial_proper_impl : Proper ((≡) ==> impl) Initial.
+Proof.
+    intros A A' (f & g & []) HA B.
+    destruct (HA B) as (h & Hh & Hunih).
+    exists (algebra_fn_compose h g); split; [by typeclasses eauto |].
+    intros h' Hh'.
+    rewrite (Hunih (algebra_fn_compose h' f)) by typeclasses eauto.
+    by rewrite <- algebra_fn_compose_assoc, algebra_iso_B0.
+Qed.
+
+End sec_sigma_algebra.
+
+Section sec_IMP_algebra.
+
+Inductive imp_sort : Type := is_A | is_B | is_C.
+
+Inductive imp_symbols : Type :=
+(* arithmetic exps *)
+| is_int : Z -> imp_symbols
+| is_var : nat -> imp_symbols
+| is_plus
+| is_minus
+| is_mul
+(* arithmetic comparators *)
+| is_eq
+| is_le
+(* boolean exps *)
+| is_true
+| is_false
+| is_not
+| is_and
+| is_or
+(* commands *)
+| is_skip
+| is_asgn : nat -> imp_symbols
+| is_seq
+| is_if
+| is_while
+.
+
+Definition imp_symbols_result (sigma : imp_symbols) : imp_sort :=
+match sigma with
+| is_int _ => is_A
+| is_var _ => is_A
+| is_plus => is_A
+| is_minus => is_A
+| is_mul => is_A
+| is_eq => is_B
+| is_le => is_B
+| is_true => is_B
+| is_false => is_B
+| is_not => is_B
+| is_and => is_B
+| is_or => is_B
+| is_skip => is_C
+| is_asgn _ => is_C
+| is_seq => is_C
+| is_if => is_C
+| is_while => is_C
+end.
+
+Definition zero_fn (a : fin 0) : imp_sort :=
+    fin_0_inv _ a.
+
+Definition if_arity : {n : nat & fin n -> imp_sort} :=
+    existT 3 (fun i =>
+    match i with
+    | 0%fin => is_B
+    | _ => is_C
+    end).
+
+Definition while_arity : {n : nat & fin n -> imp_sort} :=
+    existT 2 (fun i =>
+    match i with
+    | 0%fin => is_B
+    | _ => is_C
+    end).
+
+Definition imp_symbols_arity (sigma : imp_symbols) : {n : nat & fin n -> imp_sort} :=
+match sigma with
+| is_int _ => existT 0 zero_fn
+| is_var _ => existT 0 zero_fn
+| is_plus => existT 2 (const is_A)
+| is_minus => existT 2 (const is_A)
+| is_mul => existT 2 (const is_A)
+| is_eq => existT 2 (const is_A)
+| is_le => existT 2 (const is_A)
+| is_true => existT 0 zero_fn
+| is_false => existT 0 zero_fn
+| is_not => existT 1 (const is_B)
+| is_and => existT 2 (const is_B)
+| is_or => existT 2 (const is_B)
+| is_skip => existT 0 zero_fn
+| is_asgn _ => existT 1 (const is_A)
+| is_seq => existT 2 (const is_C)
+| is_if => if_arity
+| is_while => while_arity
+end.
+
+Definition IMP_sign : signature :=
+{|
+    sort := imp_sort;
+    symbols := imp_symbols;
+    result_sort := imp_symbols_result;
+    arity := imp_symbols_arity;
+|}.
+
+Definition IMP_term_support (s : sort IMP_sign) : Type :=
+match s with
+| is_A => AExp
+| is_B => BExp
+| is_C => Cmd
+end.
+
+Definition IMP_term_op_interp (sigma : symbols IMP_sign)
+    (tuple : support_star_helper IMP_term_support (projT2 (arity sigma))) :
+    IMP_term_support (result_sort sigma) :=
+match sigma as i
+    return
+        (support_star_helper IMP_term_support (projT2 (@arity IMP_sign i)) ->
+        IMP_term_support (@result_sort IMP_sign i))
+with
+| is_int z => fun _ => AVal z
+| is_var n => fun _ => Var n
+| is_plus => fun tuple => Plus (tuple 0%fin) (tuple 1%fin)
+| is_minus => fun tuple => Minus (tuple 0%fin) (tuple 1%fin)
+| is_mul => fun tuple => Mul (tuple 0%fin) (tuple 1%fin)
+| is_eq => fun tuple => AEq (tuple 0%fin) (tuple 1%fin)
+| is_le => fun tuple => ALe (tuple 0%fin) (tuple 1%fin)
+| is_true => fun _ => BVal true
+| is_false => fun _ => BVal false
+| is_not => fun tuple => Not (tuple 0%fin)
+| is_and => fun tuple => And (tuple 0%fin) (tuple 1%fin)
+| is_or => fun tuple => Or (tuple 0%fin) (tuple 1%fin)
+| is_skip => fun _ => Skip
+| is_asgn n => fun tuple => Asgn n (tuple 0%fin)
+| is_seq => fun tuple => Seq (tuple 0%fin) (tuple 1%fin)
+| is_if => fun tuple => If (tuple 0%fin) (tuple 1%fin) (tuple 2%fin)
+| is_while => fun tuple => While (tuple 0%fin) (tuple 1%fin)
+end
+  tuple.
+
+Definition IMP_term_algebra : algebra IMP_sign :=
+{|
+    support := IMP_term_support;
+    op_interp := IMP_term_op_interp;
+|}.
+
+Section sec_term_interp.
+
+Context
+    (A : algebra IMP_sign).
+
+Fixpoint term_interp_a (a : AExp) : support A is_A :=
+match a with
+| AVal n => op_interp A (is_int n) (fin_0_inv _)
+| Var x => op_interp A (is_var x) (fin_0_inv _)
+| Plus a1 a2 =>
+    op_interp A is_plus
+        (fun i =>
+            match i with
+            | 0%fin => term_interp_a a1
+            | _ => term_interp_a a2
+            end)
+| Minus a1 a2 =>
+    op_interp A is_minus
+        (fun i =>
+            match i with
+            | 0%fin => term_interp_a a1
+            | _ => term_interp_a a2
+            end)
+| Mul a1 a2 =>
+    op_interp A is_mul
+        (fun i =>
+            match i with
+            | 0%fin => term_interp_a a1
+            | _ => term_interp_a a2
+            end)
+end.
+
+Fixpoint term_interp_b (b : BExp) : support A is_B :=
+match b with
+| BVal true => op_interp A is_true (fin_0_inv _)
+| BVal false => op_interp A is_false (fin_0_inv _)
+| AEq a1 a2 =>
+    op_interp A is_eq
+        (fun i =>
+            match i with
+            | 0%fin => term_interp_a a1
+            | _ => term_interp_a a2
+            end)
+| ALe a1 a2 =>
+    op_interp A is_le
+        (fun i =>
+            match i with
+            | 0%fin => term_interp_a a1
+            | _ => term_interp_a a2
+            end)
+| Not b => op_interp A is_not (const (term_interp_b b))
+| And b1 b2 =>
+    op_interp A is_and
+        (fun i =>
+            match i with
+            | 0%fin => term_interp_b b1
+            | _ => term_interp_b b2
+            end)
+| Or b1 b2 =>
+    op_interp A is_or
+        (fun i =>
+            match i with
+            | 0%fin => term_interp_b b1
+            | _ => term_interp_b b2
+            end)
+end.
+
+Definition term_interp_if
+    (b : support A is_B) (c1 c2 : support A is_C) : support A is_C.
+Proof.
+    eapply (op_interp A is_if).
+    intro i; cbn in *.
+    destruct i as [| []] eqn: Hi.
+    - exact b.
+    - exact c1.
+    - exact c2.
+Defined.
+
+Definition term_interp_while
+    (b : support A is_B) (c : support A is_C) : support A is_C.
+Proof.
+    eapply (op_interp A is_while).
+    intro i; cbn in *.
+    destruct i.
+    - exact b.
+    - exact c.
+Defined.
+
+Fixpoint term_interp_c (c : Cmd) : support A is_C :=
+match c with
+| Skip => op_interp A is_skip (fin_0_inv _)
+| Asgn x a => op_interp A (is_asgn x) (const (term_interp_a a))
+| Seq c1 c2 =>
+    op_interp A is_seq
+        (fun i =>
+            match i with
+            | 0%fin => term_interp_c c1
+            | _ => term_interp_c c2
+            end)
+| If b c1 c2 =>
+    term_interp_if (term_interp_b b) (term_interp_c c1) (term_interp_c c2)
+| While b c =>
+    term_interp_while (term_interp_b b) (term_interp_c c)
+end.
+
+End sec_term_interp.
+
+Definition IMP_denot_support (s : sort IMP_sign) : Type :=
+match s with
+| is_A => State -> Z
+| is_B => State -> bool
+| is_C => Ensemble (State * State)
+end.
+
+Definition IMP_denot_op_interp (sigma : symbols IMP_sign)
+    (tuple : support_star_helper IMP_denot_support (projT2 (arity sigma))) :
+    IMP_denot_support (result_sort sigma) :=
+match sigma as i
+    return
+        (support_star_helper IMP_denot_support (projT2 (@arity IMP_sign i)) ->
+        IMP_denot_support (@result_sort IMP_sign i))
+with
+| is_int z => fun _ => const z
+| is_var n => fun _ sigma => sigma n
+| is_plus => fun tuple sigma => (tuple 0%fin sigma + tuple 1%fin sigma)%Z
+| is_minus => fun tuple sigma => (tuple 0%fin sigma - tuple 1%fin sigma)%Z
+| is_mul => fun tuple sigma => (tuple 0%fin sigma * tuple 1%fin sigma)%Z
+| is_eq => fun tuple sigma => bool_decide (tuple 0%fin sigma = tuple 1%fin sigma)%Z
+| is_le => fun tuple sigma => bool_decide (tuple 0%fin sigma <= tuple 1%fin sigma)%Z
+| is_true => fun _ => const true
+| is_false => fun _ => const false
+| is_not => fun tuple sigma => negb (tuple 0%fin sigma)
+| is_and => fun tuple sigma => andb (tuple 0%fin sigma) (tuple 1%fin sigma)
+| is_or => fun tuple sigma => orb (tuple 0%fin sigma) (tuple 1%fin sigma)
+| is_skip => fun _ => delta
+| is_asgn n => fun tuple => denot_asgn n (tuple 0%fin)
+| is_seq => fun tuple => fwd_relation_composition (tuple 0%fin) (tuple 1%fin)
+| is_if => fun tuple => relation_selector (tuple 0%fin) (tuple 1%fin) (tuple 2%fin)
+| is_while => fun tuple => lfp (while_step (tuple 0%fin) (tuple 1%fin))
+end
+  tuple.
+
+Definition IMP_denot_algebra : algebra IMP_sign :=
+{|
+    support := IMP_denot_support;
+    op_interp := IMP_denot_op_interp;
+|}.
+
+End sec_IMP_algebra.
